README.md
@@ -10,4 +10,10 @@
   + [x] Perm
   + [x] Sort
   + [x] SearchTree
+  + [x] Redblack
 - [ ] slf
+
+# Comments
+lf: you will learn basic rocq (induction), proof objects, simple imperative programs
+plf: you will learn more tactics, hoare logic, small-step semantics, type systems and proofs of type safety
+vfa: you will learn algorithms (insertion sort) and data structures (search trees, red-black trees) in rocq and their correctness proofs. you will also learn extraction of ocaml programs from rocq developments. you will learn automation of proofs using match goal.
